theory/Utils/Distributions.v
@@ -198,6 +198,21 @@ Proof.
   auto.
 Qed.
 
+Lemma dist_comm {X Y} (P : X -> Y -> Prop) (m1 : dist X) (m2 : dist Y) :
+  dist_lift (fun y => dist_lift (fun x => P x y) m1) m2 ->
+  dist_lift (fun x => dist_lift (P x) m2) m1.
+Proof.
+  destruct m1 as [m1 m1_law].
+  destruct m2 as [m2 m2_law].
+  simpl; clear m1_law m2_law.
+  repeat rewrite Forall_forall.
+  intros.
+  rewrite Forall_forall; intros.
+  apply H in H1.
+  rewrite Forall_forall in H1.
+  apply H1; auto.
+Qed.
+
 Global Instance Pred_Dist_Lift : PredLift dist :=
   {|
     plift := @dist_lift;
@@ -206,6 +221,7 @@ Global Instance Pred_Dist_Lift : PredLift dist :=
     plift_weaken := @dist_lift_weaken;
     plift_split := @dist_split;
     plift_true := @dist_true;
+    plift_comm := @dist_comm;
   |}.
 
 Lemma coin_flip_triv :
